---
title: "Gauss-Hermite quadrature: solutions"
format: html
---

1. $x_1 = -\sqrt{3}, x_2 = 0, x_3 = \sqrt{3}$

2. 

$$w_1 = \int \limits_{-\infty}^\infty \dfrac{(x - x_2)(x - x_3)}{(x_1 - x_2)(x_1 - x_3)} e^{-\frac{1}{2}x^2} dx$$
$$= \dfrac{1}{(x_1 - x_2)(x_1 - x_3)} \int \limits_{-\infty}^\infty (x^2 - (x_2 + x_3)x + x_2 x_3) e^{-\frac{1}{2}x^2} dx$$

Now, using the normal kernel we know that
$$\int \limits_{-\infty}^\infty x^2 e^{-\frac{1}{2}x^2} dx = \sqrt{2\pi} \mathbb{E}[X^2] = \sqrt{2\pi}$$
where $X \sim N(0, 1)$. Similarly,
$$\int \limits_{-\infty}^\infty x e^{-\frac{1}{2}x^2} dx = \sqrt{2\pi} \mathbb{E}[X] = 0$$
$$\int \limits_{-\infty}^\infty e^{-\frac{1}{2}x^2} dx = \sqrt{2\pi}$$

Thus,

$$w_1 = \dfrac{\sqrt{2\pi}}{(x_1 - x_2)(x_1 - x_3)} \left(1 + x_2x_3 \right)$$
Substituting $x_1, x_2, x_3$ from question 1 we get

$$w_1 = \frac{\sqrt{2\pi}}{(-\sqrt{3})(-2\sqrt{3})} = \frac{1}{3}\sqrt{\frac{\pi}{2}}$$

3.

```{r}
f <- function(x){
  x^2 / sqrt(2*pi)
}

nodes <- c(-sqrt(3), 0, sqrt(3))
weights <- c(1/3 * sqrt(pi/2), 2/3*sqrt(2*pi), 1/3 * sqrt(pi/2))
sum(weights * f(nodes))
```

Note that the calculation is **exact**, because $2 \times 3 - 1 = 5 \geq 4$. 